src/high/resources/bumpers.v
@@ -33,6 +33,16 @@ Section bumpers.
     encode_bumper bumper (encode s) = Some (encode (bumper s)).
   Proof. rewrite /encode_bumper. rewrite decode_encode. done. Qed.
 
+  (* An encoded bumper returns some encoded value then that encoded value will
+  also result in some other encoded bumper again. This represents that encoded
+  bumpers take "valid" encodings to "valid" encodings. *)
+  Lemma encode_bumper_bump_to_valid bumper e e' :
+    encode_bumper bumper e = Some e' → is_Some (encode_bumper bumper e').
+  Proof.
+    intros (s' & ? & encodeEq)%encode_bumper_Some_decode.
+    rewrite <- encodeEq. rewrite encode_bumper_encode. done.
+  Qed.
+
 End bumpers.
 
 Section own_encoded_bumpers.
